theories/core/utp_pred.thy
@@ -7,278 +7,10 @@
 header {* Predicates *}
 
 theory utp_pred
-imports utp_synonyms utp_value utp_sorts utp_var
+imports utp_binding
 begin
 
-subsection {* Value Compatibility *}
-
-(* Can the given value be placed into the given variable? *)
-definition var_compat :: "'VALUE \<Rightarrow> 'VALUE VAR \<Rightarrow> bool" (infix "\<rhd>" 50) where
-"v \<rhd> x \<equiv> v : type x \<and> (control x \<longrightarrow> \<D> v)"
-
-lemma var_compat_intros [simp,intro]:
-  "\<lbrakk> v : type x; \<D> v \<rbrakk> \<Longrightarrow> v \<rhd> x"
-  "\<lbrakk> v : type x; \<not> control x \<rbrakk> \<Longrightarrow> v \<rhd> x"
-  by (simp_all add:var_compat_def)
-
-lemma var_compat_cases [elim]:
-  "\<lbrakk> v \<rhd> x; \<lbrakk> v : type x; \<D> v \<rbrakk> \<Longrightarrow> P
-          ; \<lbrakk> v : type x; \<not> control x \<rbrakk> \<Longrightarrow> P \<rbrakk> \<Longrightarrow> P"
-  by (auto simp add:var_compat_def)
-
-subsection {* Bindings *}
-
-text {* We require bindings to be well-typed. *}
-
-definition "WF_BINDING \<equiv> {b . \<forall> v. b v \<rhd> v}"
-
-subsubsection {* Binding Theorems *}
-
-theorem WF_BINDING_exists :
-"\<exists> b . b \<in> WF_BINDING"
-apply (rule_tac x = "(\<lambda> v . SOME x . x : (type v) \<and> \<D> x)" in exI)
-apply (auto simp add: WF_BINDING_def)
-apply (rule someI2_ex)
-apply (rule type_non_empty_elim)
-apply (auto)
-done
-
-(* Some attempt to convert the above proof into ISAR. *)
-
-(*
-theorem WF_BINDING_exists :
-"\<exists> b . b \<in> WF_BINDING"
-apply (rule_tac x = "(\<lambda> v . SOME x . x : (type v))" in exI)
-apply (simp add: WF_BINDING_def)
-apply (safe)
-apply (rule someI2_ex)
-proof -
-  fix v
-  have lemma1 : "\<exists>a. a : type v"
-    apply (simp only: type_non_empty)
-  done
-  then show ?thesis using lemma1
-qed
-*)
-
-
-
-subsubsection {* Binding theorems *}
-
-theorem WF_BINDING_non_empty :
-"WF_BINDING \<noteq> {}"
-apply (insert WF_BINDING_exists)
-apply (auto)
-done
-
-theorem WF_BINDING_app_compat [intro] :
-"\<lbrakk>b \<in> WF_BINDING\<rbrakk> \<Longrightarrow> (b v) \<rhd> v"
-  apply (simp add: WF_BINDING_def)
-done
-
-theorem WF_BINDING_app_type [intro] :
-"\<lbrakk>b \<in> WF_BINDING\<rbrakk> \<Longrightarrow> (b v) : (type v)"
-apply (auto simp add: WF_BINDING_def)
-done
-
-theorem WF_BINDING_app_carrier [intro] :
-"\<lbrakk>b \<in> WF_BINDING\<rbrakk> \<Longrightarrow> (b v) \<in> carrier (type v)"
-apply (simp add: WF_BINDING_app_type carrier_def)
-done
-
-theorem WF_BINDING_update1 [closure] :
-"\<lbrakk>b \<in> WF_BINDING; x \<rhd> v\<rbrakk> \<Longrightarrow>
- b(v := x) \<in> WF_BINDING"
-apply (simp add: WF_BINDING_def)
-done
-
-theorem WF_BINDING_update2 [closure] :
-"\<lbrakk>b \<in> WF_BINDING; x \<in> carrier (type v); \<not> control v\<rbrakk> \<Longrightarrow>
- b(v := x) \<in> WF_BINDING"
-apply (simp add: carrier_def closure)
-done
-
-theorem WF_BINDING_update2_control [closure] :
-"\<lbrakk>b \<in> WF_BINDING; x \<in> carrier (type v); control v; \<D> x\<rbrakk> \<Longrightarrow>
- b(v := x) \<in> WF_BINDING"
-apply (simp add: carrier_def closure)
-done
-
-theorem WF_BINDING_override [closure] :
-"\<lbrakk>b1 \<in> WF_BINDING;
- b2 \<in> WF_BINDING\<rbrakk> \<Longrightarrow>
- b1 \<oplus> b2 on vs \<in> WF_BINDING"
-apply (simp add: WF_BINDING_def)
-apply (safe)
-apply (case_tac "v \<in> vs")
-apply (auto simp add:override_on_def)
-done
-
-theorem WF_BINDING_control_defined [defined]:
-"\<lbrakk> b \<in> WF_BINDING; control v \<rbrakk> \<Longrightarrow> \<D> (b v)"
-  by (auto simp add:WF_BINDING_def)
-
-typedef (open) 'VALUE WF_BINDING = "WF_BINDING :: 'VALUE BINDING set"
-  by (simp add: WF_BINDING_exists)
-
-declare Rep_WF_BINDING [simp]
-declare Rep_WF_BINDING_inverse [simp]
-declare Abs_WF_BINDING_inverse [simp]
-
-lemma Rep_WF_BINDING_intro [intro]:
-  "Rep_WF_BINDING x = Rep_WF_BINDING y \<Longrightarrow> x = y"
-  by (simp add:Rep_WF_BINDING_inject)
-
-lemma Rep_WF_BINDING_elim [elim]:
-  "\<lbrakk> x = y; Rep_WF_BINDING x = Rep_WF_BINDING y \<Longrightarrow> P \<rbrakk> \<Longrightarrow> P"
-  by (auto)
-
-notation Rep_WF_BINDING ("\<langle>_\<rangle>\<^sub>b")
-
-text {* Binding Equivalence *}
-
-definition binding_equiv ::
-  "'VALUE WF_BINDING \<Rightarrow>
-   'VALUE WF_BINDING \<Rightarrow>
-   ('VALUE VAR set) \<Rightarrow> bool" where
-"(binding_equiv b1 b2 a) \<longleftrightarrow> (\<forall> x \<in> a . \<langle>b1\<rangle>\<^sub>bx = \<langle>b2\<rangle>\<^sub>bx)"
-
-notation binding_equiv ("_ \<cong> _ on _")
-
-setup_lifting type_definition_WF_BINDING
-
-lift_definition binding_override_on ::
-  "'VALUE WF_BINDING \<Rightarrow>
-   'VALUE WF_BINDING \<Rightarrow>
-   'VALUE VAR set \<Rightarrow>
-   'VALUE WF_BINDING" ("_ \<oplus>\<^sub>b _ on _" [56, 56, 0] 55) is "override_on"
-  apply (simp add: WF_BINDING_def)
-  apply (safe)
-  apply (case_tac "v \<in> set")
-  apply (auto)
-done
-
-declare binding_override_on.rep_eq [simp]
-
-definition binding_upd :: 
-  "'VALUE WF_BINDING \<Rightarrow>
-   'VALUE VAR \<Rightarrow>
-   'VALUE \<Rightarrow>
-   'VALUE WF_BINDING" where
-"binding_upd b x v = Abs_WF_BINDING (fun_upd \<langle>b\<rangle>\<^sub>b x v)"
-
-nonterminal bupdbinds and bupdbind
-
-syntax
-  "_bupdbind" :: "['a, 'a] => bupdbind"               ("(2_ :=\<^sub>b/ _)")
-  ""         :: "bupdbind => bupdbinds"               ("_")
-  "_bupdbinds":: "[bupdbind, bupdbinds] => bupdbinds" ("_,/ _")
-  "_BUpdate"  :: "['a, bupdbinds] => 'a"              ("_/'((_)')" [1000, 0] 900)
-
-translations
-  "_BUpdate f (_bupdbinds b bs)" == "_BUpdate (_BUpdate f b) bs"
-  "f(x:=\<^sub>by)" == "CONST binding_upd f x y"
-
-lemma binding_type [simp, typing, intro]: "t = type x \<Longrightarrow> \<langle>b\<rangle>\<^sub>bx : t"
-  apply (insert Rep_WF_BINDING[of b])
-  apply (auto simp add:WF_BINDING_def)
-done
-
-lemma binding_compat [simp, intro]: "\<langle>b\<rangle>\<^sub>bx \<rhd> x"
-  by auto
-
-lemma binding_value_alt [simp, intro]: 
-  "\<lbrakk> type x = type x'; control x = control x' \<rbrakk> \<Longrightarrow> \<langle>b\<rangle>\<^sub>bx \<rhd> x'"
-  by (auto simp add:var_compat_def intro: defined)
-
-lemma Rep_WF_BINDING_rep_eq [simp]:
-  "\<lbrakk> v \<rhd> x \<rbrakk> \<Longrightarrow> \<langle>binding_upd b x v\<rangle>\<^sub>b = fun_upd \<langle>b\<rangle>\<^sub>b x v"
-  apply (simp add:var_compat_def)
-  apply (subgoal_tac "\<langle>b\<rangle>\<^sub>b(x := v) \<in> WF_BINDING")
-  apply (simp_all add: binding_upd_def WF_BINDING_def)
-  apply (auto intro:defined closure)
-done
-
-lemma binding_eq_iff: "f = g = (\<forall>x. \<langle>f\<rangle>\<^sub>b x = \<langle>g\<rangle>\<^sub>b x)"
-  by (auto)
-
-lemma binding_upd_idem_iff: "y \<rhd> x \<Longrightarrow> (f(x:=\<^sub>by) = f) = (\<langle>f\<rangle>\<^sub>b x = y)"
-  by (force simp add: fun_upd_idem_iff var_compat_def)
-
-lemma binding_upd_idem: "\<lbrakk> y \<rhd> x \<rbrakk> \<Longrightarrow> \<langle>f\<rangle>\<^sub>b x = y ==> f(x:=\<^sub>by) = f"
-  by (simp add: binding_upd_idem_iff)
-
-lemma binding_upd_triv [iff]: "f(x :=\<^sub>b \<langle>f\<rangle>\<^sub>b x) = f"
-  by (simp add: binding_upd_idem)
-
-lemma binding_upd_apply [simp]: "y \<rhd> x \<Longrightarrow> \<langle>f(x:=\<^sub>by)\<rangle>\<^sub>b z = (if z=x then y else \<langle>f\<rangle>\<^sub>b z)"
-  by (simp)
-
-lemma binding_upd_upd [simp]: 
-  "\<lbrakk> y \<rhd> x; z \<rhd> x \<rbrakk> \<Longrightarrow> f(x:=\<^sub>by,x:=\<^sub>bz) = f(x:=\<^sub>bz)"
-  by (simp add: binding_eq_iff)
-
-lemma binding_upd_twist: 
-  "\<lbrakk> b \<rhd> a; d \<rhd> c; a ~= c \<rbrakk> \<Longrightarrow> (m(a:=\<^sub>bb))(c:=\<^sub>bd) = (m(c:=\<^sub>bd))(a:=\<^sub>bb)"
-  by (force)
-
-theorem binding_override_on_eq :
-"f1 \<oplus>\<^sub>b g1 on a = f2 \<oplus>\<^sub>b g2 on a \<longleftrightarrow>
- (\<forall> x . x \<in> a \<longrightarrow> \<langle>g1\<rangle>\<^sub>bx = \<langle>g2\<rangle>\<^sub>bx) \<and>
- (\<forall> x . x \<notin> a \<longrightarrow> \<langle>f1\<rangle>\<^sub>bx = \<langle>f2\<rangle>\<^sub>bx)"
-  by (simp add:binding_override_on_def Abs_WF_BINDING_inject closure override_on_eq)
-
-(* Transfer override theorems *)
-lemma binding_override_simps [simp]:
-  "(f \<oplus>\<^sub>b g on vs1) \<oplus>\<^sub>b g on vs2 = f \<oplus>\<^sub>b g on (vs1 \<union> vs2)"
-  "f \<oplus>\<^sub>b f on vs = f"
-  "(f \<oplus>\<^sub>b g on vs) \<oplus>\<^sub>b h on vs = f \<oplus>\<^sub>b h on vs"
-  "f \<oplus>\<^sub>b (g \<oplus>\<^sub>b h on a) on a = f \<oplus>\<^sub>b h on a"
-  "f \<oplus>\<^sub>b (g \<oplus>\<^sub>b f on b) on a = f \<oplus>\<^sub>b g on a - b"
-  "f \<oplus>\<^sub>b (f \<oplus>\<^sub>b g on a) on b = f \<oplus>\<^sub>b g on a \<inter> b"
-  "f \<oplus>\<^sub>b g on (insert x xs) = f(x :=\<^sub>b \<langle>g\<rangle>\<^sub>bx) \<oplus>\<^sub>b g on xs - {x}"
-  "v \<rhd> x \<Longrightarrow> (f \<oplus>\<^sub>b g on a)(x :=\<^sub>b v) = f(x :=\<^sub>b v) \<oplus>\<^sub>b g on (a - {x})"
-  "x \<in> vs2 \<Longrightarrow> \<langle>f \<oplus>\<^sub>b g on vs1 - vs2\<rangle>\<^sub>bx = \<langle>f\<rangle>\<^sub>bx"
-  "f \<oplus>\<^sub>b g on VAR = g"
-  "f \<oplus>\<^sub>b g on {} = f"
-  apply (auto simp add:override_on_assoc override_on_singleton override_on_chain)
-  apply (auto intro!: Rep_WF_BINDING_intro)
-  apply (metis Un_empty_left Un_insert_left insert_Diff_single override_on_chain override_on_singleton)
-done
-
-lemma binding_override_singleton:
-  "(f \<oplus>\<^sub>b g on {x}) = f(x :=\<^sub>b \<langle>g\<rangle>\<^sub>bx)"
-  by (auto)
-
-lemma binding_override_assoc:
-  "(f \<oplus>\<^sub>b g on a) \<oplus>\<^sub>b h on b = f \<oplus>\<^sub>b (g \<oplus>\<^sub>b h on b) on (a \<union> b)"
-  by (auto simp add:override_on_assoc)
-
-lemma binding_override_subset: 
-"\<lbrakk> f = f \<oplus>\<^sub>b g on vs1; vs2 \<subseteq> vs1 \<rbrakk> \<Longrightarrow> f = f \<oplus>\<^sub>b g on vs2"
-  by (force simp add:override_on_subset)
-
-lemma binding_override_reorder:
-"\<lbrakk> a \<inter> b = {} \<rbrakk> \<Longrightarrow>
- (f \<oplus>\<^sub>b g on a) \<oplus>\<^sub>b h on b = (f \<oplus>\<^sub>b h on b) \<oplus>\<^sub>b g on a"
-  apply (rule Rep_WF_BINDING_intro)
-  apply (simp)
-  apply (drule_tac f="\<langle>f\<rangle>\<^sub>b" and g="\<langle>g\<rangle>\<^sub>b" and h="\<langle>h\<rangle>\<^sub>b" in override_on_reorder)
-  apply (simp)
-done
-
-lemma binding_override_equiv [simp]:
-  "b1 \<cong> b2 on vs \<Longrightarrow> b1 \<oplus>\<^sub>b b2 on vs = b1"
-  by (force simp add:override_on_def binding_equiv_def)
-
-lemma binding_override_upd [simp]:
-  "\<lbrakk> x \<in> vs; v \<rhd> x \<rbrakk> \<Longrightarrow> b1 \<oplus>\<^sub>b b2(x :=\<^sub>b v) on vs = b1(x :=\<^sub>b v) \<oplus>\<^sub>b b2 on (vs - {x})"
-  by (force simp add:override_on_def)
-
-lemma binding_upd_simps [simp]:
-  "\<lbrakk> v1 \<rhd> x; v2 \<rhd> x \<rbrakk> \<Longrightarrow> b(x :=\<^sub>b v1, x :=\<^sub>b v2) = b(x :=\<^sub>b v2)"
-  "b(x :=\<^sub>b \<langle>b\<rangle>\<^sub>b x) = b"
-  by (auto)
+subsection {* Predicates *}
 
 text {* Binding Predicates *}
 
@@ -289,17 +21,12 @@ definition WF_BINDING_PRED ::
   "'VALUE VAR set \<Rightarrow> 'VALUE WF_BINDING_PRED set" where
 "WF_BINDING_PRED vs = {f . \<forall> b1 b2 . b1 \<cong> b2 on vs \<longrightarrow> f b1 = f b2}"
 
-subsection {* Predicates *}
-
 definition WF_PREDICATE :: "'VALUE PREDICATE set" where
 "WF_PREDICATE = Pow WF_BINDING"
 
 typedef (open) 'VALUE WF_PREDICATE = "UNIV :: 'VALUE WF_BINDING set set"
 morphisms destPRED mkPRED
   by (auto)
-
-print_theorems
-
 
 declare destPRED [simp]
 declare destPRED_inverse [simp]
@@ -313,6 +40,10 @@ lemma destPRED_elim [elim]:
   "\<lbrakk> x = y; destPRED x = destPRED y \<Longrightarrow> P \<rbrakk> \<Longrightarrow> P"
   by (auto)
 
+text {* The lifting package allows us to define operators on a typedef
+by lifting operators on the underlying type. The following command sets
+up the @{term "WF_PREDICATE"} type for lifting. *}
+
 setup_lifting type_definition_WF_PREDICATE
 
 subsection {* Functions *}
@@ -321,12 +52,16 @@ type_synonym 'VALUE WF_FUNCTION = "'VALUE WF_PREDICATE \<Rightarrow> 'VALUE WF_P
 
 subsection {* Operators *}
 
+text {* We define many of these operators by lifting. Each lift
+definition requires a name, type, underlying operator and a proof
+that the operator is closed under the charateristic set. *}
+
 subsubsection {* Shallow Lifting *}
 
 lift_definition LiftP ::
   "('VALUE WF_BINDING \<Rightarrow> bool) \<Rightarrow>
    'VALUE WF_PREDICATE" is 
-  "Collect :: ('VALUE WF_BINDING \<Rightarrow> bool) \<Rightarrow> 'VALUE WF_BINDING set" done
+  "Collect :: ('VALUE WF_BINDING \<Rightarrow> bool) \<Rightarrow> 'VALUE WF_BINDING set" .
 
 subsubsection {* Equality *}
 
@@ -340,12 +75,12 @@ notation EqualsP (infix "=p" 210)
 subsubsection {* True and False *}
 
 lift_definition TrueP :: "'VALUE WF_PREDICATE" 
-  is "UNIV :: 'VALUE WF_BINDING set" done
+  is "UNIV :: 'VALUE WF_BINDING set" .
 
 notation TrueP ("true")
 
 lift_definition FalseP :: "'VALUE WF_PREDICATE" 
-is "{} :: 'VALUE WF_BINDING set" done
+is "{} :: 'VALUE WF_BINDING set" .
 
 notation FalseP ("false")
 
@@ -354,7 +89,7 @@ subsubsection {* Logical Connectives *}
 lift_definition NotP ::
   "'VALUE WF_PREDICATE \<Rightarrow>
    'VALUE WF_PREDICATE" 
-is "uminus" done
+is "uminus" .
 
 notation NotP ("\<not>p _" [190] 190)
 
@@ -362,8 +97,7 @@ lift_definition AndP ::
   "'VALUE WF_PREDICATE \<Rightarrow>
    'VALUE WF_PREDICATE \<Rightarrow>
    'VALUE WF_PREDICATE" 
-is "op \<inter> :: 'VALUE WF_BINDING set \<Rightarrow> 'VALUE WF_BINDING set \<Rightarrow> 'VALUE WF_BINDING set"
-done
+is "op \<inter> :: 'VALUE WF_BINDING set \<Rightarrow> 'VALUE WF_BINDING set \<Rightarrow> 'VALUE WF_BINDING set" .
 
 notation AndP (infixr "\<and>p" 180)
 
@@ -371,8 +105,7 @@ lift_definition OrP ::
   "'VALUE WF_PREDICATE \<Rightarrow>
    'VALUE WF_PREDICATE \<Rightarrow>
    'VALUE WF_PREDICATE" 
-is "op \<union> :: 'VALUE WF_BINDING set \<Rightarrow> 'VALUE WF_BINDING set \<Rightarrow> 'VALUE WF_BINDING set"
-done
+is "op \<union> :: 'VALUE WF_BINDING set \<Rightarrow> 'VALUE WF_BINDING set \<Rightarrow> 'VALUE WF_BINDING set" .
 
 notation OrP (infixr "\<or>p" 170)
 
@@ -398,8 +131,7 @@ lift_definition ExistsP ::
   "('VALUE VAR set) \<Rightarrow>
    'VALUE WF_PREDICATE \<Rightarrow>
    'VALUE WF_PREDICATE" is
-"\<lambda> vs p. {b1 \<oplus>\<^sub>b b2 on vs | b1 b2. b1 \<in> p}"
-done
+"\<lambda> vs p. {b1 \<oplus>\<^sub>b b2 on vs | b1 b2. b1 \<in> p}" .
 
 notation ExistsP ("(\<exists>p _ ./ _)" [0, 10] 10)
 
