theories/core/utp_rel.thy
@@ -7,7 +7,7 @@
 header {* Relations *}
 
 theory utp_rel
-imports utp_pred utp_expr utp_subst utp_unrest "../tactics/utp_expr_tac"
+imports utp_pred utp_expr utp_rename utp_unrest "../tactics/utp_expr_tac"
 begin
 
 subsection {* Composable Bindings *}
@@ -21,29 +21,29 @@ definition COMPOSABLE_BINDINGS ::
 "COMPOSABLE_BINDINGS =
  {(b1, b2) . (\<forall> v \<in> UNDASHED . \<langle>b1\<rangle>\<^sub>b(dash v) = \<langle>b2\<rangle>\<^sub>b v) \<and> b1 \<cong> b2 on NON_REL_VAR}"
 
-subsection {* Substitutions *}
+subsection {* Renamings *}
 
-text {* The substitution @{term "SS"} swaps dashed and undashed variables. *}
+text {* The renaming @{term "SS"} swaps dashed and undashed variables. *}
 
-lift_definition SS :: "'VALUE VAR_SUBST" is
+lift_definition SS :: "'VALUE VAR_RENAME" is
 "(\<lambda> v .
    if v \<in> UNDASHED then (dash v) else
    if v \<in> DASHED then (undash v) else v)"
-  by (auto simp add:VAR_SUBST_def bij_def inj_on_def)
+  by (auto simp add:VAR_RENAME_def bij_def inj_on_def)
 
-lift_definition SS1 :: "'VALUE VAR_SUBST" is
+lift_definition SS1 :: "'VALUE VAR_RENAME" is
 "(\<lambda> v .
    if (v \<in> DASHED) then (dash v) else
    if (v \<in> DASHED_TWICE) then (undash v) else v)"
-  apply (auto simp add: VAR_SUBST_def bij_def inj_on_def)
+  apply (auto simp add: VAR_RENAME_def bij_def inj_on_def)
   apply (smt DASHED_dash_DASHED_TWICE DASHED_not_DASHED_TWICE IntI imageI mem_Collect_eq undash_dash)
 done
 
-lift_definition SS2 :: "'VALUE VAR_SUBST" is
+lift_definition SS2 :: "'VALUE VAR_RENAME" is
 "(\<lambda> v .
    if v \<in> UNDASHED then dash (dash v) else
    if v \<in> DASHED_TWICE then undash (undash v) else v)"
-  apply (auto simp add: VAR_SUBST_def bij_def inj_on_def)
+  apply (auto simp add: VAR_RENAME_def bij_def inj_on_def)
   apply (metis (lifting) DASHED_TWICE_undash_DASHED dash_undash_DASHED dash_undash_DASHED_TWICE)
   apply (auto simp add: image_def)[1]
   apply (drule_tac x="dash (dash x)" in bspec) back
@@ -113,7 +113,7 @@ notation AssignR ("_ :=p\<^bsub>_ \<^esub>_" [190] 190)
 
 subsection {* Theorems *}
 
-subsubsection {* Substitution Theorems *}
+subsubsection {* Renaming Theorems *}
 
 text {* Theorems for @{term SS} *}
 
@@ -145,14 +145,14 @@ theorems SS_simps =
   SS_DASHED_TWICE_app
   SS_ident_app
 
-theorem SS_VAR_SUBST_ON [closure] :
-"SS \<in> VAR_SUBST_ON (UNDASHED \<union> DASHED)"
-  by (simp add: VAR_SUBST_ON_def SS.rep_eq)
+theorem SS_VAR_RENAME_ON [closure] :
+"SS \<in> VAR_RENAME_ON (UNDASHED \<union> DASHED)"
+  by (simp add: VAR_RENAME_ON_def SS.rep_eq)
 
-theorem SS_VAR_SUBST_INV [closure] :
-"SS \<in> VAR_SUBST_INV"
-apply (simp add: VAR_SUBST_INV_def)
-apply (rule Rep_VAR_SUBST_intro)
+theorem SS_VAR_RENAME_INV [closure] :
+"SS \<in> VAR_RENAME_INV"
+apply (simp add: VAR_RENAME_INV_def)
+apply (rule Rep_VAR_RENAME_intro)
 apply (simp add:SS.rep_eq)
 apply (rule sym [OF inv_equality])
 apply (auto)
@@ -160,18 +160,17 @@ done
 
 theorem SS_inv [simp] :
 "inv\<^sub>s SS = SS"
-apply (insert SS_VAR_SUBST_INV)
-apply (simp add: VAR_SUBST_INV_def VAR_SUBST_def)
-apply (metis (lifting) SS_VAR_SUBST_INV VAR_SUBST_INV_inv)
+apply (insert SS_VAR_RENAME_INV)
+apply (simp add: VAR_RENAME_INV_def VAR_RENAME_def)
+apply (metis (lifting) SS_VAR_RENAME_INV VAR_RENAME_INV_inv)
 done
 
 theorem SS_inv' [simp] :
 "inv \<langle>SS\<rangle>\<^sub>s = \<langle>SS\<rangle>\<^sub>s"
   apply (insert SS_inv)
-  apply (erule Rep_VAR_SUBST_elim)
-  apply (simp only: subst_inv_rep_eq)
+  apply (erule Rep_VAR_RENAME_elim)
+  apply (simp only: rename_inv_rep_eq)
 done
-
 
 theorem SS_DASHED_member :
 "x \<in> DASHED \<Longrightarrow> \<not> \<langle>SS\<rangle>\<^sub>s x \<in> DASHED"
@@ -201,16 +200,16 @@ theorem SS1_ident_app :
 apply (simp add: SS1.rep_eq)
 done
 
-theorem SS1_VAR_SUBST_ON [closure] :
-"SS1 \<in> VAR_SUBST_ON (DASHED \<union> DASHED_TWICE)"
-apply (simp add: VAR_SUBST_ON_def)
+theorem SS1_VAR_RENAME_ON [closure] :
+"SS1 \<in> VAR_RENAME_ON (DASHED \<union> DASHED_TWICE)"
+apply (simp add: VAR_RENAME_ON_def)
 apply (simp add: SS1.rep_eq)
 done
 
-theorem SS1_VAR_SUBST_INV [closure] :
-"SS1 \<in> VAR_SUBST_INV"
-apply (simp add: VAR_SUBST_INV_def)
-apply (rule Rep_VAR_SUBST_intro)
+theorem SS1_VAR_RENAME_INV [closure] :
+"SS1 \<in> VAR_RENAME_INV"
+apply (simp add: VAR_RENAME_INV_def)
+apply (rule Rep_VAR_RENAME_intro)
 apply (simp add:SS1.rep_eq)
 apply (rule sym [OF inv_equality])
 apply (auto)
@@ -218,16 +217,16 @@ done
 
 theorem SS1_inv [simp] :
 "inv\<^sub>s SS1 = SS1"
-apply (insert SS1_VAR_SUBST_INV)
-apply (simp add: VAR_SUBST_INV_def VAR_SUBST_def)
-apply (metis (lifting) SS1_VAR_SUBST_INV VAR_SUBST_INV_inv)
+apply (insert SS1_VAR_RENAME_INV)
+apply (simp add: VAR_RENAME_INV_def VAR_RENAME_def)
+apply (metis (lifting) SS1_VAR_RENAME_INV VAR_RENAME_INV_inv)
 done
 
 theorem SS1_inv' [simp] :
 "inv \<langle>SS1\<rangle>\<^sub>s = \<langle>SS1\<rangle>\<^sub>s"
   apply (insert SS1_inv)
-  apply (erule Rep_VAR_SUBST_elim)
-  apply (simp only: subst_inv_rep_eq)
+  apply (erule Rep_VAR_RENAME_elim)
+  apply (simp only: rename_inv_rep_eq)
 done
 
 theorem SS1_UNDASHED_DASHED_image :
@@ -266,14 +265,14 @@ theorem SS2_ident_app :
 apply (simp add: SS2.rep_eq)
 done
 
-theorem SS2_VAR_SUBST_ON [closure] :
-"SS2 \<in> VAR_SUBST_ON (UNDASHED \<union> DASHED_TWICE)"
-  by (simp add: VAR_SUBST_ON_def SS2.rep_eq)
+theorem SS2_VAR_RENAME_ON [closure] :
+"SS2 \<in> VAR_RENAME_ON (UNDASHED \<union> DASHED_TWICE)"
+  by (simp add: VAR_RENAME_ON_def SS2.rep_eq)
 
-theorem SS2_VAR_SUBST_INV [closure] :
-"SS2 \<in> VAR_SUBST_INV"
-  apply (simp add: VAR_SUBST_INV_def)
-  apply (rule Rep_VAR_SUBST_intro)
+theorem SS2_VAR_RENAME_INV [closure] :
+"SS2 \<in> VAR_RENAME_INV"
+  apply (simp add: VAR_RENAME_INV_def)
+  apply (rule Rep_VAR_RENAME_intro)
   apply (simp add:SS2.rep_eq)
   apply (rule sym [OF inv_equality])
   apply (auto)
@@ -281,16 +280,16 @@ done
 
 theorem SS2_inv [simp] :
 "inv\<^sub>s SS2 = SS2"
-apply (insert SS2_VAR_SUBST_INV)
-apply (simp add: VAR_SUBST_INV_def VAR_SUBST_def)
-apply (metis (lifting) SS2_VAR_SUBST_INV VAR_SUBST_INV_inv)
+apply (insert SS2_VAR_RENAME_INV)
+apply (simp add: VAR_RENAME_INV_def VAR_RENAME_def)
+apply (metis (lifting) SS2_VAR_RENAME_INV VAR_RENAME_INV_inv)
 done
 
 theorem SS2_inv' [simp] :
 "inv \<langle>SS2\<rangle>\<^sub>s = \<langle>SS2\<rangle>\<^sub>s"
   apply (insert SS2_inv)
-  apply (erule Rep_VAR_SUBST_elim)
-  apply (simp only: subst_inv_rep_eq)
+  apply (erule Rep_VAR_RENAME_elim)
+  apply (simp only: rename_inv_rep_eq)
 done
 
 theorem SS2_UNDASHED_DASHED_image :
@@ -385,12 +384,12 @@ subsection {* Validation of Soundness *}
 
 lemma SemiR_algebraic_lemma1 :
 "\<lbrakk>(b1, b2) \<in> COMPOSABLE_BINDINGS\<rbrakk> \<Longrightarrow>
-  CompB ((b1 \<oplus>\<^sub>b b2 on DASHED) \<oplus>\<^sub>b (SubstB SS1 b1) on DASHED_TWICE) SS1 =
-   b1 \<oplus>\<^sub>b (SubstB SS1 b2) on DASHED_TWICE"
+  CompB ((b1 \<oplus>\<^sub>b b2 on DASHED) \<oplus>\<^sub>b (RenameB SS1 b1) on DASHED_TWICE) SS1 =
+   b1 \<oplus>\<^sub>b (RenameB SS1 b2) on DASHED_TWICE"
 apply (rule Rep_WF_BINDING_intro)
 apply (simp add:CompB_rep_eq)
 apply (rule ext)
-apply (simp add: SubstB_def closure)
+apply (simp add: RenameB_def closure)
 apply (case_tac "x \<in> UNDASHED")
 apply (simp add: SS1_simps SS2_simps)
 apply (case_tac "x \<in> DASHED")
@@ -402,12 +401,12 @@ done
 
 lemma SemiR_algebraic_lemma2 :
 "\<lbrakk>(b1, b2) \<in> COMPOSABLE_BINDINGS\<rbrakk> \<Longrightarrow>
- CompB ((b1 \<oplus>\<^sub>b b2 on DASHED) \<oplus>\<^sub>b (SubstB SS1 b1) on DASHED_TWICE) SS2 =
-   b2 \<oplus>\<^sub>b (SubstB SS2 b1) on DASHED_TWICE"
+ CompB ((b1 \<oplus>\<^sub>b b2 on DASHED) \<oplus>\<^sub>b (RenameB SS1 b1) on DASHED_TWICE) SS2 =
+   b2 \<oplus>\<^sub>b (RenameB SS2 b1) on DASHED_TWICE"
 apply (rule Rep_WF_BINDING_intro)
 apply (simp)
 apply (rule ext)
-apply (simp add: SubstB_def closure)
+apply (simp add: RenameB_def closure)
 apply (case_tac "x \<in> UNDASHED")
 apply (simp add: SS1_simps SS2_simps)
 apply (simp add: COMPOSABLE_BINDINGS_dash)
@@ -430,9 +429,9 @@ apply (simp add: SemiR_def)
 apply (safe)
 -- {* Subgoal 1 *}
 apply (rule_tac x =
-  "SubstB (inv\<^sub>s SS1) (b \<oplus>\<^sub>b b' on DASHED_TWICE) \<oplus>\<^sub>b b on DASHED_TWICE" in exI)
+  "RenameB (inv\<^sub>s SS1) (b \<oplus>\<^sub>b b' on DASHED_TWICE) \<oplus>\<^sub>b b on DASHED_TWICE" in exI)
 apply (rule_tac x =
-  "SubstB (inv\<^sub>s SS2) (b \<oplus>\<^sub>b b' on DASHED_TWICE) \<oplus>\<^sub>b b on DASHED_TWICE" in exI)
+  "RenameB (inv\<^sub>s SS2) (b \<oplus>\<^sub>b b' on DASHED_TWICE) \<oplus>\<^sub>b b on DASHED_TWICE" in exI)
 apply (safe)
 -- {* Subgoal 1.1 *}
 apply (simp add: closure)
@@ -440,17 +439,17 @@ apply (rule Rep_WF_BINDING_intro)
 apply (rule ext)
 apply (case_tac "x \<in> DASHED")
 apply (simp add: SS1_simps SS2_simps)
-apply (simp add: SubstB_def)
+apply (simp add: RenameB_def)
 apply (simp add: SS1_simps SS2_simps)
 apply (case_tac "x \<in> DASHED_TWICE")
 apply (simp add: SS1_simps SS2_simps)
-apply (simp add: SS1_simps SS2_simps SubstB_def)
+apply (simp add: SS1_simps SS2_simps RenameB_def)
 -- {* Subgoal 1.2 *}
 apply (auto intro: UNREST_binding_override) [1]
 -- {* Subgoal 1.3 *}
 apply (auto intro: UNREST_binding_override) [1]
 -- {* Subgoal 1.3 *}
-apply (simp add: SubstB_def closure)
+apply (simp add: RenameB_def closure)
 apply (simp add: COMPOSABLE_BINDINGS_def)
 apply (safe)
 apply (simp add: SS1_simps SS2_simps)
@@ -462,8 +461,8 @@ apply (case_tac "x \<in> DASHED_TWICE")
 apply (simp add: SS1_simps SS2_simps)
 apply (simp add: SS1_simps SS2_simps)
 -- {* Subgoal 2 *}
-apply (simp add: SubstB_def closure)
-apply (rule_tac x = "SubstB SS1 b1" in exI)
+apply (simp add: RenameB_def closure)
+apply (rule_tac x = "RenameB SS1 b1" in exI)
 apply (rule conjI)
 -- {* Subgoal 2.1 *}
 apply (simp add: SemiR_algebraic_lemma1)
@@ -483,13 +482,13 @@ lemma UNREST_SemiR:
   apply (simp add:SemiR_algebraic)
   apply (rule UNREST_ExistsP_alt)
   apply (rule UNREST_AndP_alt)
-  apply (rule_tac ?vs1.0="VAR - vs1" in UNREST_SubstP_alt)
+  apply (rule_tac ?vs1.0="VAR - vs1" in UNREST_RenameP_alt)
   apply (blast intro:unrest)
   apply (force)
-  apply (rule_tac ?vs1.0="VAR - vs2" in UNREST_SubstP_alt)
+  apply (rule_tac ?vs1.0="VAR - vs2" in UNREST_RenameP_alt)
   apply (blast intro:unrest)  
   apply (force)
-  apply (simp add:inj_on_image_set_diff[OF Rep_VAR_SUBST_inj])
+  apply (simp add:inj_on_image_set_diff[OF Rep_VAR_RENAME_inj])
   apply (simp add:SS1_UNDASHED_DASHED_image[simplified])
   apply (simp add:SS2_UNDASHED_DASHED_image[simplified])
   apply (simp add:VAR_def)
